more work on linker spec.

sepcomp/linking2.v
@@ -11,7 +11,10 @@ Set Implicit Arguments.
   after Ssreflect eqtype.*)
 Require Import compcert.common.AST.    (*for typ*)
 Require Import compcert.common.Values. (*for val*)
+Require Import compcert.common.Globalenvs. 
 Require Import compcert.lib.Integers.
+
+Require Import ZArith.
 
 Module Stack.
 Definition t (T : Type) := seq T.
@@ -26,175 +29,345 @@ Definition updStack (newStack : seq T) := newStack.
 Definition push (stack: Stack.t T) (t: T) := updStack [:: t & stack].
 Definition peek (stack: Stack.t T) : option T :=
   if stack is [:: topT & rest] then Some topT else None.
-Definition pop  (stack: Stack.t T) : seq T := 
-  if stack is [:: topT & rest] then rest else [::].
+Definition pop  (stack: Stack.t T) : Stack.t T := behead stack.
 Definition empty : Stack.t T := [::].
 
 Definition nonempty : pred (Stack.t T) := 
   [pred s | if s is [::] then false else true].
 
-Lemma peek_push (t : T) (stack : Stack.t T) : peek (push stack t) = Some t.
-Proof. by []. Qed.
-
-Lemma pop_push (t : T) (stack : Stack.t T) : pop (push stack t) = stack.
-Proof. by []. Qed.
-
 Lemma peek_nonempty (stack : Stack.t T) : 
   nonempty stack -> exists t, peek stack = Some t.
 Proof. by case: stack=>// a l _; exists a. Qed.
 
+Lemma all_pop (stack : Stack.t T) p : all p stack -> all p (pop stack).
+Proof. by case: stack=>//= a l; move/andP=> [H1 H2]. Qed.
+
 End stackDefs. End StackDefs.
 
 (* Export push, pop, empty, nonempty, push_pop, pop_nonempty *)
+
 Definition push      := StackDefs.push.
 Definition pop       := StackDefs.pop.
 Definition peek      := StackDefs.peek.
 Definition empty     := StackDefs.empty.
 Definition nonempty  := StackDefs.nonempty.
-Definition peek_push := StackDefs.peek_push.
-Definition pop_push  := StackDefs.pop_push.
 Definition peek_nonempty := StackDefs.peek_nonempty.
+Definition all_pop   := StackDefs.all_pop.
 
 Implicit Arguments empty [T].
 
+(* Dummy signatures, external functions, and core semantics *)
+
+Definition dummy_sig := mksignature [::] None.
+
+Definition dummy_ef  := EF_external xH dummy_sig.
+
+Program Definition dummy_coreSem {G C M: Type} : @CoreSemantics G C M :=
+  Build_CoreSemantics G C M
+    (fun _ _ _ => None)
+    (fun _ => Some (dummy_ef, dummy_sig, [::]))
+    (fun _ _ => None)
+    (fun _ => None)
+    (fun _ _ _ _ _ => False)
+    _ _ _ _.
+Next Obligation. by []. Qed.
+
+Axiom dummy_genv: forall F V, Genv.t F V. (*FIXME*)
+
 (* Cores are runtime execution units *)
+
 Module Core.
-Record t (G M: Type) := mk
-  { C   : Type
-  ; sem : @CoreSemantics G C M
-  ; ge  :  G
+Record t (M: Type) := mk
+  { F   : Type
+  ; V   : Type
+  ; C   : Type
+  ; sem : @CoreSemantics (Genv.t F V) C M
+  ; ge  :  Genv.t F V
   ; c   :> C
   }.
 
-Definition upd {G M: Type} (core : t G M) (newC : core.(C)) :=
-  {| C     := core.(C)
+Definition upd {M: Type} (core : t M) (newC : core.(C)) :=
+  {| F     := core.(F)
+   ; V     := core.(V)
+   ; C     := core.(C)
    ; sem   := core.(sem)
    ; ge    := core.(ge)
    ; c     := newC 
    |}.
 
-Program Definition nullCoreSem {G C M: Type} : @CoreSemantics G C M :=
-  Build_CoreSemantics G C M
-    (fun _ _ _ => None)
-    (fun _ => None)
-    (fun _ _ => None)
-    (fun _ => None)
-    (fun _ _ _ _ _ => False)
-    _ _ _ _.
+Definition dummy {M: Type} : t M := mk dummy_coreSem (dummy_genv unit unit) tt.
 
-Definition null {G M: Type} (ge: G) : t G M := mk nullCoreSem ge tt.
 End Core.
 
-Record linker (G M: Type) (N: nat) := mkLinker
-  (* The first two fields of this record are static configuration data:  
-     -[cores] is a function from module id's ('I_n, or integers in the range [0..n-1]) 
-      to genvs and core semantics, with existentially quantified core type [C]. 
-     -[fn_tbl] maps external function id's to module id's
-     [stack] is used to maintain a stack of cores, at runtime. *)
-  { cores : 'I_N  -> (G * {C: Type & @CoreSemantics G C M})%type
-  ; fn_tbl: ident -> option 'I_N
-  ; stack : Stack.t (Core.t G M)
+Definition atExternal {M: Type} (c: Core.t M) :=
+  let: (Core.mk F V C coreSem ge c) := c in
+  if at_external coreSem c is Some (ef, dep_sig, args) then true
+  else false.
+
+(* Linker invariants: 
+   -1: all cores except the topmost one are at_external 
+   -2: the call stack always contains at least one core *)
+
+Definition wf_callStack {M: Type} (stk: Stack.t (Core.t M)) :=
+  [&& all [pred c | atExternal c] (pop stk) & size stk > 0].
+
+(* Call stacks are [stack]s satisfying the [wf_callStack] invariant. *)
+
+Module CallStack.
+Record t (M: Type) : Type := mk
+  { callStack :> Stack.t (Core.t M)
+  ; _         :  wf_callStack callStack 
   }.
 
-Implicit Arguments mkLinker [G M N].
+End CallStack.
+
+Section callStackDefs.
+Context {M: Type} (stack: CallStack.t M).
+
+Import CallStack.
+
+Definition callStackSize := size stack.(callStack).
+
+Program Definition singl_callStack (core: Core.t M) := 
+  CallStack.mk [:: core] _.
+
+Definition dummy_callStack := singl_callStack Core.dummy.
+
+Lemma callStack_wf : wf_callStack stack.
+Proof. by case: stack. Qed.
+
+Lemma callStack_ext : all [pred c | atExternal c] (pop stack).
+Proof. by move: callStack_wf; move/andP=> [H1 H2]. Qed.
+
+Lemma callStack_size : callStackSize > 0.
+Proof. by move: callStack_wf; move/andP=> [H1 H2]. Qed.
+
+End callStackDefs.
+
+Module Payload.
+Record t (M: Type) := mk
+  { F   : Type
+  ; V   : Type
+  ; ge  : Genv.t F V
+  ; C   : Type
+  ; coreSem : @CoreSemantics (Genv.t F V) C M
+  ; c   : C
+  }.
+
+Definition dummy (M: Type) := 
+  @mk M unit unit (dummy_genv _ _) unit dummy_coreSem tt.
+
+End Payload.
+
+(* The first two fields of this record are static configuration data:  
+   -[cores] is a function from module id's ('I_n, or integers in the range [0..n-1]) 
+    to genvs and core semantics, with existentially quantified core type [C]. 
+   -[fn_tbl] maps external function id's to module id's
+   [stack] is used to maintain a stack of cores, at runtime. 
+   Parameter [N] is the number of static modules in the program. *)
+
+Record linker (M: Type) (N: nat) := mkLinker
+  { cores : 'I_N  -> Payload.t M
+  ; fn_tbl: ident -> option 'I_N
+  ; stack : CallStack.t M
+  }.
+
+Implicit Arguments mkLinker [M N].
 
 Section linkerDefs.
-Context {G M: Type} {N: nat} (l: linker G M N).
+Context {M: Type} {N: nat} (l: linker M N).
 
-Definition updStack (newStack: Stack.t (Core.t G M)) :=
+Import CallStack. (*for coercion [callStack]*)
+
+Definition dummy_linker := 
+  mkLinker (fun _ : 'I_N => Payload.dummy M) (fun id => None) dummy_callStack.
+
+Section emptyLinker.
+Variables (my_cores: 'I_N -> Payload.t M) (my_fun_tbl : ident -> option 'I_N).
+
+Definition empty_linker := mkLinker my_cores my_fun_tbl dummy_callStack.
+
+Lemma empty_linker_ext :
+  all [pred c | atExternal c] empty_linker.(stack).(CallStack.callStack).
+Proof. by []. Qed.  
+
+End emptyLinker.
+
+Definition updStack (newStack: CallStack.t M) :=
   {| cores  := l.(cores)
    ; fn_tbl := l.(fn_tbl)
    ; stack  := newStack
   |}.
 
-Definition pushCore (newCore: Core.t G M) := 
-  updStack (push l.(stack) newCore).
+(* [inContext]: The top core on the call stack has a return context *)
 
-Definition popCore := 
-  updStack (pop l.(stack)).
+Definition inContext (l0 : linker M N) := callStackSize l0.(stack) > 1.
+
+(* [updCore]: Replace the top core on the call stack with [newCore] *)
+
+Program Definition updCore (newCore: Core.t M) := 
+  updStack (CallStack.mk (push (pop l.(stack)) newCore) _).  
+Next Obligation. apply/andP; split=>/=; last by []; by apply: callStack_ext. Qed.
+
+(* [pushCore]: Push a new core onto the call stack.  
+   Succeeds only if all cores are currently at_external. *)
+
+Program Definition pushCore 
+  (newCore: Core.t M) (_ : all [pred c | atExternal c] l.(stack).(callStack)) := 
+  updStack (CallStack.mk (push l.(stack) newCore) _).
+Next Obligation. by rewrite/wf_callStack; apply/andP; split. Qed.
+
+(* [popCore]: Pop the top core on the call stack.  
+   Succeeds only if the top core is running in a return context. *)
+
+Lemma inContext_wf (stk : Stack.t (Core.t M)) : 
+  size stk > 1 -> wf_callStack stk -> wf_callStack (pop stk).
+Proof.
+rewrite/wf_callStack=> H1; move/andP=> [H2 H3]; apply/andP; split.
+by apply: all_pop.
+by move: H1 H2 H3; case: stk.
+Qed.
+
+Program Definition popCore : option (linker M N) := 
+  (match inContext l as pf return (pf = inContext l -> option (linker M N)) with
+    | true => fun pf => 
+        Some (updStack (CallStack.mk (pop l.(stack)) (inContext_wf _ _ _)))
+    | false => fun pf => None
+  end) Logic.eq_refl.
+Next Obligation. by apply: callStack_wf. Qed.
 
 Definition peekCore := peek l.(stack).
 
-Definition emptyStack := if l.(stack) is [::] then true else false.
+Definition emptyStack := if l.(stack).(callStack) is [::] then true else false.
 
 Lemma peekCore_nempty c : peekCore = Some c -> emptyStack = false.
-Proof. by rewrite/peekCore/peek/emptyStack/StackDefs.peek; case: (stack l). Qed.
+Proof. by rewrite/peekCore/peek/emptyStack/StackDefs.peek; case: (callStack _). Qed.
 
-Definition initCore (ix: 'I_N) (v: val) (args: list val): option (Core.t G M) :=
-  let: (ge, (existT C coreSem)) := l.(cores) ix in
+Definition initCore (ix: 'I_N) (v: val) (args: list val): option (Core.t M) :=
+  let: Payload.mk F V ge C coreSem c := l.(cores) ix in
   if initial_core coreSem ge v args is Some c then Some (Core.mk coreSem ge c)
   else None.
 
 End linkerDefs.
 
-Lemma peek_pushCore {G M: Type} {N: nat} c (l: linker G M N) : 
-  peekCore (pushCore l c) = Some c.
-Proof. by []. Qed.
-
 (* The linking semantics *)
 
 Module LinkerSem. Section linkerSem.
-Variables G M: Type.
-Variable  N  : nat.  (* Number of modules *)
-Variable my_cores : 'I_N  -> (G * {C: Type & @CoreSemantics G C M})%type.
+Variables M : Type.
+Variable  N : nat.  (* Number of (compile-time) modules *)
+Variable my_cores : 'I_N  -> Payload.t M.
 Variable my_fn_tbl: ident -> option 'I_N.
 
-Definition initial_core (ge: G) (v: val) (args: list val): option (linker G M N) :=
-  Some (mkLinker my_cores my_fn_tbl empty). 
+(* [handle id l args] looks up function id [id] in function table [l.fn_tbl], 
+   producing an optional module index [ix : 'I_N].  The index is used to 
+   construct a new core to handle the call to function [id]. The new core 
+   is pushed onto the call stack. *)
 
-Definition at_external0 (l: linker G M N) :=
+Section handle.
+Variables (id: ident) (l: linker M N) (args: list val).
+
+Import CallStack.
+
+Definition handle :=
+  (match all [pred c | atExternal c] l.(stack).(callStack) as pf 
+        return (pf = all [pred c | atExternal c] l.(stack).(callStack) 
+               -> option (linker M N)) with
+    | true => fun pf => 
+        if l.(fn_tbl) id is Some ix then
+        if initCore l ix (Vptr id Int.zero) args is Some c 
+          then Some (pushCore l c (Logic.eq_sym pf))
+        else None else None
+    | false => fun _ => None
+  end) Logic.eq_refl.
+
+End handle.
+
+Definition initial_core (tt: unit) (v: val) (args: list val)
+  : option (linker M N) :=
+  if v is Vptr id ofs then handle id (empty_linker my_cores my_fn_tbl) args 
+  else None.
+
+(* Is the running core at_external? *)
+
+Definition at_external0 (l: linker M N) :=
   let: mc := peekCore l in
   if mc is Some c then at_external (Core.sem c) (Core.c c) else None.
 
-Definition halted0 (l: linker G M N) :=
+(* Is the running core halted? *)
+
+Definition halted0 (l: linker M N) :=
   let: mc := peekCore l in
   if mc is Some c then halted (Core.sem c) (Core.c c) else None.
 
-Definition corestep0 (ge: G) (l: linker G M N) (m: M) (l': linker G M N) (m': M) := 
+(* Lift a running core step to linker step *)
+
+Definition corestep0 (l: linker M N) (m: M) (l': linker M N) (m': M) := 
   let: mc := peekCore l in
   if mc is Some c then 
-    exists c', corestep (Core.sem c) ge (Core.c c) m c' m'
-            /\ l' = pushCore l (Core.upd c c')
+    exists c', corestep (Core.sem c) (Core.ge c) (Core.c c) m c' m'
+            /\ l' = updCore l (Core.upd c c')
   else False.
-
-Definition handle (id: ident) (l: linker G M N) (args: list val) :=
-  if l.(fn_tbl) id is Some ix then
-    if initCore l ix (Vptr id Int.zero) args is Some c then Some (pushCore l c) else None
-  else None.
 
 Definition fun_id (ef: external_function) : option ident :=
   if ef is (EF_external id sig) then Some id else None.
 
-Definition at_external (l: linker G M N) :=
+(* The linker is [at_external] whenever the top core is [at_external] and 
+   the [id] of the called external function isn't handleable by any 
+   compilation unit. *)
+
+Definition at_external (l: linker M N) :=
   if at_external0 l is Some (ef, dep_sig, args) 
     then if fun_id ef is Some id then
          if handle id l args is None then Some (ef, dep_sig, args) else None
          else None
   else at_external0 l.
 
-Definition after_external (mv: option val) (l: linker G M N) :=
+Definition after_external (mv: option val) (l: linker M N) :=
   let: mc := peekCore l in
   if mc is Some c then 
     if after_external (Core.sem c) mv (Core.c c) is Some c' then 
-      Some (pushCore (popCore l) (Core.upd c c'))
+      Some (updCore l (Core.upd c c'))
     else None
   else None.
 
-Definition halted (l: linker G M N) := 
-  if emptyStack l then Some (Vint Int.zero) else None.
+(* The linker is [halted] when the last core on the call stack is halted. *)
 
-Definition corestep (ge: G) (l: linker G M N) (m: M) (l': linker G M N) (m': M) := 
-  if halted0 l is Some rv 
-    then if after_external (Some rv) (popCore l) is Some l'' then l'=l'' else False
-  else 
-  if at_external0 l is Some (ef, dep_sig, args) 
-    then if fun_id ef is Some id then 
-         if handle id l args is Some l'' then l'=l'' else False
-         else False
-  else corestep0 ge l m l' m'.
+Definition halted (l: linker M N) := 
+  if ~~inContext l then 
+  if halted0 l is Some rv then Some rv
+  else None else None.
 
-Lemma corestep_not_at_external0 ge m c m' c' :
-  corestep0 ge c m c' m' -> at_external0 c = None.
+
+Definition corestep (ge: unit) (l: linker M N) (m: M) (l': linker M N) (m': M) := 
+  (* 1- The running core takes a step, or *)
+  corestep0 l m l' m' \/
+
+  (* 2- We're in a function call context. In this case, the running core is either *)
+  (if inContext l then 
+
+      (* 3- at_external, in which case we push a core onto the stack to handle 
+         the external function call (or this is not possible because no module 
+         handles the external function id, in which case the entire linker is 
+         at_external) *)
+
+      if at_external0 l is Some (ef, dep_sig, args) then
+      if fun_id ef is Some id then
+      if handle id l args is Some l'' then l'=l'' else False else False
+      else 
+
+      (* 4- or halted, in which case we pop the halted core from the call stack
+         and inject its return value into the caller's corestate. *)
+
+      if halted0 l is Some rv then
+      if popCore l is Some l0 then 
+      if after_external (Some rv) l0 is Some l'' then l'=l'' 
+      else False else False else False
+
+   else False).
+
+
+Lemma corestep_not_at_external0 m c m' c' :
+  corestep0 c m c' m' -> at_external0 c = None.
 Proof.
 rewrite/corestep0/at_external0; case: (peekCore c)=>// a [newCore][H1 H2].
 by apply corestep_not_at_external in H1.
@@ -207,58 +380,48 @@ rewrite/at_external0/halted0; case: (peekCore c); last by right.
 by move=> a; apply: at_external_halted_excl.
 Qed.
 
-Lemma corestep_not_halted0 ge m c m' c' :
-  corestep0 ge c m c' m' -> halted c = None.
+Lemma corestep_not_halted0 m c m' c' :
+  corestep0 c m c' m' -> halted c = None.
 Proof.
 rewrite/corestep0/halted; case Heq: (peekCore c)=>//[a].
-by move=> [newCore [H1 H2]]; rewrite (@peekCore_nempty _ _ _ c a).
+move=> [newCore [H1 H2]]. 
+case Hcx: (~~ inContext _)=>//; case Hht: (halted0 _)=>//.
+by move: Hht; apply corestep_not_halted in H1; rewrite/halted0 Heq H1.
 Qed.
 
 Lemma corestep_not_at_external ge m c m' c' :
   corestep ge c m c' m' -> at_external c = None.
 Proof.
 rewrite/corestep/at_external. 
+move=> [H|H]; first by move: H; move/corestep_not_at_external0=> ->.
+move: H; case Hcx: (inContext _)=>//.
 case Heq: (at_external0 c)=>//[[[ef sig] args]].
-case Hht: (halted0 c)=>//. 
-case Hat: (after_external _ _)=>// _.
-by case: (at_external_halted_excl0 c)=> [H|H]; congruence.
-by move: Heq; case: (fun_id ef)=>// id H; case: (handle _ _ _).
-Qed.
-
-Lemma halted0_not_halted c rv :
-  halted0 c = Some rv -> halted c = None.
-Proof.
-rewrite/halted0/halted.
-by case Heq: (peekCore c)=>//[a] H; rewrite (@peekCore_nempty _ _ _ c a).
+move: Heq; case: (at_external_halted_excl0 c)=> [H|H]; first by rewrite H.
+by move=> H2; case: (fun_id ef)=>// id; case: (handle _ _ _).
 Qed.
 
 Lemma at_external0_not_halted c x :
   at_external0 c = Some x -> halted c = None.
 Proof.
-rewrite/at_external0/halted.
-by case Heq: (peekCore c)=>//[a] H; rewrite (@peekCore_nempty _ _ _ c a).
+case: (at_external_halted_excl0 c); rewrite/at_external0/halted.
+by case Heq: (peekCore c)=>//[a] ->.
+move=> H; case Heq: (peekCore c)=>//[a]. 
+by case Hcx: (~~ inContext _)=>//; rewrite H.
 Qed.
 
 Lemma corestep_not_halted ge m c m' c' :
   corestep ge c m c' m' -> halted c = None.
-Proof.
-rewrite/corestep/halted. 
-case Hht: (halted0 c)=>//. 
-by move=> _; apply: (halted0_not_halted _ Hht).
-case Hat: (at_external0 c)=>// H. 
-by apply: (at_external0_not_halted _ Hat).
-by apply: (corestep_not_halted0 _ _ _ _ _ H).
+Proof. 
+rewrite/corestep/halted.
+move=> [H|H]; first by move: H; move/corestep_not_halted0.
+by move: H; case Hcx: (inContext _).
 Qed.
 
 Lemma at_external_halted_excl c :
   at_external c = None \/ halted c = None.
 Proof.
-rewrite/at_external/halted; case: (peekCore c).
-move=> a; case Hat: (at_external0 c)=>//; 
+rewrite/at_external/halted; case Hat: (at_external0 c)=>//; 
 first by right; apply: (at_external0_not_halted _ Hat). 
-by left.
-case Hat: (at_external0 c)=>//; 
-first by right; apply: (at_external0_not_halted _ Hat).
 by left.
 Qed.
 
@@ -269,13 +432,12 @@ rewrite/after_external/at_external; case: (peekCore c)=>// a.
 case Heq: (core_semantics.after_external _ _ _)=>//.
 inversion 1; subst.
 case Hat: (at_external0 _)=>//[[[ef sig] args]].
-move: Hat; rewrite/at_external0.
-rewrite peek_pushCore=> H2.
+move: Hat; rewrite/at_external0=>/= H2.
 by apply after_at_external_excl in Heq; rewrite Heq in H2; congruence.
 Qed.
 
 Definition coreSem := 
-  Build_CoreSemantics G (linker G M N) M 
+  Build_CoreSemantics unit (linker M N) M 
     initial_core
     at_external
     after_external
